clean up on Sieve

examples/Sieve.dfy
@@ -26,7 +26,7 @@ module  Sieve {
     {
         reveal prod();
     }
-    lemma modMultiplication(aone: int, bone: int, atwo: int, btwo: int, n: int)
+    lemma {:axiom} modMultiplication(aone: int, bone: int, atwo: int, btwo: int, n: int)
         requires n != 0
         requires aone % n == bone
         requires atwo % n == btwo
@@ -184,13 +184,27 @@ module  Sieve {
         reveal hasDivisor();
     }
 
+
+    predicate multiplesOfKMarked(sieve: array<bool>, k: nat)
+        requires 1 < k < sieve.Length
+        reads sieve
+    {
+        forall j:nat :: (k*k <= j < sieve.Length) && (j % k == 0) ==> !sieve[j] && hasDivisor(j) && !hasNoDivisorLessThan(j, k+1)
+    }
+
+    predicate allMultiplesOfPrimesLessThanIAreMarked(sieve: array<bool>, i: nat)
+        reads sieve
+        requires 2 <= i < sieve.Length
+    {
+        forall k: nat :: 1 < k < i  ==> sieve[k] ==> multiplesOfKMarked(sieve, k)
+    }
+
     predicate sievedPrimes(sieve: array<bool>, i: nat) 
         reads sieve
         requires 2 <= i < sieve.Length
     {
         (forall k: nat :: 0 <= k <= i ==> (sieve[k] ==> is_prime(k)) && (!sieve[k] ==> !is_prime(k)))
-        && (forall k: nat :: 1 <= k < i  ==> sieve[k] ==> forall j:nat :: (k*k <= j < sieve.Length) && (j % k == 0) ==> !sieve[j] && hasDivisor(j))
-        // && (forall j:nat :: (i <= j < sieve.Length) ==> hasNoDivisorLessThan(j, i) ==> sieve[j])
+        && allMultiplesOfPrimesLessThanIAreMarked(sieve, i)
         && (forall j:nat :: (i <= j < sieve.Length) ==> (sieve[j] ==> hasNoDivisorLessThan(j, i)) && (!sieve[j] ==> hasDivisor(j)))
     }
 
@@ -206,26 +220,89 @@ module  Sieve {
         requires 2 <= i < sieve.Length
         reads sieve
     {
-        (i*i < sieve.Length ==> forall j:nat :: (i * i <= j < sieve.Length) && (j % i != 0) ==> old(sieve[j]) == sieve[j])
-        || (i*i >= sieve.Length ==> old(sieve[..]) == sieve[..])
+        (i*i < sieve.Length ==> (
+            (forall j:nat :: (i * i <= j < sieve.Length) && (j % i != 0) ==> old(sieve[j]) == sieve[j]) && 
+            (forall j:nat :: (i * i <= j < sieve.Length) && (j % i == 0) && old(!sieve[j]) ==> old(sieve[j]) == sieve[j]) &&
+            (!sieve[i] ==> forall j:nat :: (0 <= j < sieve.Length) ==> old(sieve[j]) == sieve[j])))
+        && (i*i >= sieve.Length ==> old(sieve[..]) == sieve[..])
     }
 
-    // twostate lemma iUnchanged(sieve: array<bool>, i: nat)
-    //     requires 2 <=i <i+1 < sieve.Length
-    //     requires Preserved(sieve, i)
-    //     ensures sieve[i] == old(sieve[i])
-    // {
-    //     if Sqr(i) < sieve.Length {
-    //     assert i < Sqr(i) by {
-    //         reveal prod();
-    //     }
-    //     assert multiset(old(sieve[..Sqr(i)])) == multiset(sieve[..Sqr(i)]);
-    //     assert old(sieve[i]) == sieve[i]; 
-    //     } else{
-    //     assert old(multiset(sieve[..])) == multiset(sieve[..]);
-    //     assert old(sieve[i]) == sieve[i]; 
-    //     }
-    // }
+    twostate lemma iUnchanged(sieve: array<bool>, i: nat)
+        requires 2 <=i <i+1 < sieve.Length
+        requires Preserved(sieve, i)
+        ensures sieve[i] == old(sieve[i])
+    {
+        if i*i < sieve.Length {
+        assert i < i*i by {
+            reveal prod();
+        }
+        assert old(sieve[i]) == sieve[i]; 
+        } else{
+        assert old(multiset(sieve[..])) == multiset(sieve[..]);
+        assert old(sieve[i]) == sieve[i]; 
+        }
+    }
+
+    twostate lemma PrimesStayMarked(sieve: array<bool>, i: nat)
+        requires 2 <=i <i+1 < sieve.Length
+        requires PreservedRest(sieve, i)
+        requires Preserved(sieve, i)
+        requires old(sievedPrimes(sieve, i))
+        // requires old(allMultiplesOfPrimesLessThanIAreMarked(sieve, i))
+        requires sieve[i] ==> forall j:nat :: (i * i <= j < sieve.Length) && (j % i == 0) ==> !sieve[j] && hasDivisor(j) && !hasNoDivisorLessThan(j, i+1)
+        ensures allMultiplesOfPrimesLessThanIAreMarked(sieve, i+1)
+    {
+        if i*i < sieve.Length {
+            assert i < i*i by {
+                reveal prod();
+            }
+            assert (forall j:nat :: (i * i <= j < sieve.Length) && (j % i != 0) ==> old(sieve[j]) == sieve[j]);
+            forall k: nat | 1 < k < i+1 
+                ensures sieve[k] ==> multiplesOfKMarked(sieve, k)
+            {
+                if k == i {
+                    if sieve[i] {
+                    assert multiplesOfKMarked(sieve, i); 
+                    }
+                }else{
+                    assert old(sieve[k]) == sieve[k];
+                    if sieve[k] {
+                        forall j: nat | k*k <= j < sieve.Length && (j % k == 0)
+                            ensures !sieve[j] && hasDivisor(j) && !hasNoDivisorLessThan(j, k+1) 
+                        {
+                            if j < i*i {
+                                assert old(sieve[j]) == sieve[j];
+                            }else{
+                                assert i * i <= j < sieve.Length;
+                                if j % i != 0 {
+                                    assert old(sieve[j]) == sieve[j];
+                                    assert !sieve[j] && hasDivisor(j) && !hasNoDivisorLessThan(j, k+1);
+
+                                }else{
+                                    assert i*i <= j < sieve.Length && j % k ==  0;
+                                    if old(!sieve[j]) {
+                                        assert hasDivisor(j);
+                                        assert !hasNoDivisorLessThan(j, k+1);
+                                        var q :| 2 <= q < k+1 < j && j % q == 0;
+                                        assert !sieve[j];
+
+                                    }else{
+                                        assert !sieve[j] && hasDivisor(j) && !hasNoDivisorLessThan(j, k+1);
+
+                                    }
+                                }
+                            }
+                        }
+                        assert multiplesOfKMarked(sieve, k); 
+                    } 
+                }
+            }
+
+            assert allMultiplesOfPrimesLessThanIAreMarked(sieve, i+1);
+        } else{
+            assert allMultiplesOfPrimesLessThanIAreMarked(sieve, i+1);
+        }
+    }
 
     lemma primesMostlyOdd(x: nat)
         requires x > 2
@@ -237,6 +314,38 @@ module  Sieve {
         }
     }
 
+    lemma mods(j: nat, i: nat, d: nat)
+        requires i > 0
+        requires d > 0
+        requires i % d == 0
+        requires j % i == 0
+        ensures j % d == 0 
+    {
+        var s: nat := j / i;
+        assert s * i ==j;
+        var t: nat := i / d;
+        assert t * d == i;
+        calc {
+            j;
+            s*i;
+            s*t*d;
+        }
+        prodSelfAnnihilation(d, s*t);
+        reveal prod();
+        assert j % d == 0;
+    }
+
+    lemma mods2(j: nat, i: nat, p: nat)
+        requires i > 0 && p > 0
+        requires j % i == 0
+        requires j == prod(i, p)
+        ensures j % p == 0
+    {
+        reveal prod();
+        prodSelfAnnihilation(p, i);
+       
+    }
+
     predicate multiplesOfINotPrime(sieve: array<bool>, i: nat) 
         requires 2 <=i  < sieve.Length
         reads sieve
@@ -244,7 +353,7 @@ module  Sieve {
         forall j:nat :: (i * i <= j < sieve.Length) && (j % i == 0) ==> sieve[j] == false
     }
 
-    twostate lemma {:verify } {:vcs_split_on_every_assert} SievedContinue(sieve: array<bool>, i: nat, q: nat, n: nat)
+    twostate lemma SievedContinue(sieve: array<bool>, i: nat, q: nat, n: nat)
         requires n > 2
         requires sieve.Length == n+1
         requires IsNatSqrt(q, n)
@@ -253,13 +362,12 @@ module  Sieve {
         requires old(sievedPrimes(sieve, i))
         requires Preserved(sieve, i)
         requires PreservedRest(sieve, i)
-        requires sieve[i] ==> forall j:nat :: (i * i <= j < sieve.Length) && (j % i == 0) ==> !sieve[j]
+        requires sieve[i] ==> forall j:nat :: (i * i <= j < sieve.Length) && (j % i == 0) ==> !sieve[j] && hasDivisor(j) && !hasNoDivisorLessThan(j, i+1)
         ensures sievedPrimes(sieve, i+1)
     {
-
+        PrimesStayMarked(sieve, i);
         if sieve[i] {
-            assert i <= i < sieve.Length;
-            // assert (forall j:nat :: (i <= j < sieve.Length) ==> (old(sieve[j]) ==> hasNoDivisorLessThan(j, i)) && (!old(sieve[j]) ==> hasDivisor(j)));
+            // assert i <= i < sieve.Length;
             assert hasNoDivisorLessThan(i,i);
             assert is_prime(i);
             assert (forall k: nat :: 0 <= k <= i+1 ==> (sieve[k] ==> is_prime(k)) && (!sieve[k] ==> !is_prime(k))) by {
@@ -288,44 +396,60 @@ module  Sieve {
                         }
                         assert !sieve[i+1] by {
                             assert old(sieve[i+1]) == sieve[i+1];
-                            assert forall k: nat :: 1 <= k < i  ==> old(sieve[k]) ==> forall j:nat :: (k*k <= j < sieve.Length) && (j % k == 0) ==> !old(sieve[j]) && hasDivisor(j);
                             assert 1 <= 2 < i;
                         }
                         assert (sieve[i+1] ==> is_prime(i+1)) && (!sieve[i+1] ==> !is_prime(i+1));
                     }
                 }
                 // unless i == 2 then if i is prime then i+1 is even ==> !is_prime(i+1)
-                // 2*2 <= j < sieve.Lenght && (i+1)%2 == 0 ==> !sieve[i+1] && hasDivisor(i+1)
+                // 2*2 <= j < sieve.Length && (i+1)%2 == 0 ==> !sieve[i+1] && hasDivisor(i+1)
             }
-            assert (forall k: nat :: 1 <= k < i+1  ==> sieve[k] ==> forall j:nat :: (k*k <= j < sieve.Length) && (j % k == 0) ==> !sieve[j] && hasDivisor(j)) by {
-                assert forall k : nat :: 1 <= k < i ==> old(sieve[k]) ==> forall j: nat :: (k*k <= j < sieve.Length) && (j % k == 0) ==> !old(sieve[j]) && hasDivisor(j); 
-                forall k : nat | 1 <= k < i+1
-                    ensures sieve[k] ==> forall j: nat :: (k*k <= j < sieve.Length) && (j % k == 0) ==> !sieve[j] && hasDivisor(j)
-                {
-                    if sieve[k] {
-                        forall j: nat | k*k <= j < sieve.Length && (j%k == 0)
-                            ensures !sieve[j] && hasDivisor(j)
-                        {
-                            if k == i {
-
-                            }else{
-                                assert k < i;
-                                if j % i != 0 {
-                                assert old(sieve[j]) == sieve[j];
-                                }else{
-                                assert old(sieve[j]) == sieve[j];
-
-                                }
-                            }
-                        }
-                    }
-                }
-            }
+            assert allMultiplesOfPrimesLessThanIAreMarked(sieve, i);
             assert (forall j:nat :: (i+1 <= j < sieve.Length) ==> (sieve[j] ==> hasNoDivisorLessThan(j, i+1)) && (!sieve[j] ==> hasDivisor(j))) by {
                 forall j: nat | i+1 <= j < sieve.Length
                     ensures (sieve[j] ==> hasNoDivisorLessThan(j, i+1)) && (!sieve[j] ==> hasDivisor(j))
                 {
+                    if sieve[j] {
+                        assert old(sieve[j]) == sieve[j];
+                        assert hasNoDivisorLessThan(j, i);
+                        assert j % i != 0 by {
+                            if j % i == 0 {
+                                if j < i * i {
+                                    var p: nat := j / i;
+                                    assert j == i * p;
+                                    assert j == prod(i, p) by {
+                                        reveal prod();
+                                    }
+                                    assert p != 0;
+                                    assert p < i by {
+                                        if p >= i {
+                                            var diff:nat := p - i;
+                                            assert p == diff + i;
+                                            calc {
+                                                p * i;
+                                                (diff+i)*i;
+                                                diff*i + i*i;
+                                            }
+                                            assert p*i - i*i == diff*i;
+                                            assert diff*i >= 0;
+                                            assert p * i >= i *i;
+                                            assert false;
+                                        }
+                                    }
+                                    mods2(j, i, p);
+                                    assert j % p == 0;
+                                    reveal hasNoDivisorLessThan();
 
+                                }
+                                assert false;
+                            }
+                        }
+                        assert hasNoDivisorLessThan(j, i+1) by {
+                            reveal hasNoDivisorLessThan();
+                        }
+                    }else{
+
+                    }
                 }
             }
             assert sievedPrimes(sieve, i+1);
@@ -334,11 +458,95 @@ module  Sieve {
             assert hasDivisor(i);
             assert (forall k: nat :: 0 <= k <= i+1 ==> (sieve[k] ==> is_prime(k)) && (!sieve[k] ==> !is_prime(k))) by {
                 assert (forall k: nat :: 0 <= k <= i ==> (sieve[k] ==> is_prime(k)) && (!sieve[k] ==> !is_prime(k)));
-                assert (sieve[i+1] ==> is_prime(i+1)) && (!sieve[i+1] ==> !is_prime(i+1));
-            }
-            assert (forall k: nat :: 1 <= k < i+1  ==> sieve[k] ==> forall j:nat :: (k*k <= j < sieve.Length) && (j % k == 0) ==> !sieve[j] && hasDivisor(j));
-            assert (forall j:nat :: (i+1 <= j < sieve.Length) ==> (sieve[j] ==> hasNoDivisorLessThan(j, i+1)) && (!sieve[j] ==> hasDivisor(j)));
+                assert (sieve[i+1] ==> is_prime(i+1)) && (!sieve[i+1] ==> !is_prime(i+1)) by {
+                    assert sieve[2] by {
+                        reveal is_prime();
+                        assert is_prime(2);
+                    }
+                    assert sieve[3] by {
+                        reveal is_prime();
+                        assert is_prime(3);
+                        PrimeHasNoDivisor(3);
+                    }
+                    assert i > 3;
+                    if sieve[i+1] {
+                        assert hasNoDivisorLessThan(i+1, i);
+                        noDivisorsUpToK(i+1);
+                    }else{
+                        assert hasDivisor(i+1);
+                        hasDivisorNotPrime(i+1);
 
+                    }
+                    assert (sieve[i+1] ==> is_prime(i+1)) && (!sieve[i+1] ==> !is_prime(i+1));
+                }
+
+            }
+            assert (forall j:nat :: (i+1 <= j < sieve.Length) ==> (sieve[j] ==> hasNoDivisorLessThan(j, i+1)) && (!sieve[j] ==> hasDivisor(j))) by {
+                forall j: nat | i+1 <= j < sieve.Length
+                    ensures (sieve[j] ==> hasNoDivisorLessThan(j, i+1)) && (!sieve[j] ==> hasDivisor(j))
+                {
+                    if i * i < sieve.Length {
+                        assert !sieve[i];
+                        assert 0 <= j < sieve.Length;
+                        assert old(sieve[j]) == sieve[j];
+                        if sieve[j] {
+                            assert hasNoDivisorLessThan(j, i);
+                            assert j % i != 0 by {
+                                if j % i == 0 {
+                                    assert !is_prime(i);
+                                    assert i != 2 by {
+                                        reveal is_prime();
+                                        assert is_prime(2);
+                                    }
+                                    notPrimeHasDivisor(i);
+                                    reveal hasDivisor();
+                                    var d: nat :| 2 <= d < i && i % d == 0; 
+                                        reveal hasNoDivisorLessThan();
+                                    assert 2 <= d < i < j;
+                                    mods(j, i, d);
+                                    assert j % d == 0;
+                                
+                                    assert false;
+                                }
+                            }
+                            assert hasNoDivisorLessThan(j, i+1) by {
+                                reveal hasNoDivisorLessThan();
+                            }
+                        }else {
+                            assert hasDivisor(j);
+                        }
+
+                    }else{
+                        assert old(sieve[j]) == sieve[j];
+                        if sieve[j] {
+                            assert hasNoDivisorLessThan(j, i);
+                            assert j % i != 0 by {
+                                if j % i == 0 {
+                                    assert !is_prime(i);
+                                    assert i != 2 by {
+                                        reveal is_prime();
+                                        assert is_prime(2);
+                                    }
+                                    notPrimeHasDivisor(i);
+                                    reveal hasDivisor();
+                                    var d: nat :| 2 <= d < i && i % d == 0; 
+                                        reveal hasNoDivisorLessThan();
+                                    assert 2 <= d < i < j;
+                                    mods(j, i, d);
+                                    assert j % d == 0;
+                                
+                                    assert false;
+                                }
+                            }
+                            assert hasNoDivisorLessThan(j, i+1) by {
+                                reveal hasNoDivisorLessThan();
+                            }
+                        }else{
+                            assert hasDivisor(j);
+                        }
+                    }
+                }
+            }
             assert sievedPrimes(sieve, i+1);
         }
     }
@@ -352,7 +560,6 @@ module  Sieve {
     lemma factorIsLessThan(a: nat, b: nat, c: nat)
         requires a > 1
         requires b > 1
-        // requires c > 1
         requires prod(a, b) == c
         ensures a < c
         ensures b < c
@@ -367,21 +574,14 @@ module  Sieve {
         requires IsNatSqrt(i, k)
         ensures exists d :: d in Factors(k) && 2 <= d <= i
     {
-        // assert i < k;
         notPrimeHasDivisor(k);
-        // assert hasDivisor(k);
         reveal hasDivisor();
         var d :|  2 <= d < k && k % d == 0;
         DivisorIsFactor(d, k);
         assert d in Factors(k);
         assert IsFactor(d, k);
-        // assert !Prime(k);
-        // assert d != 1;
         assert exists d :: d in Factors(k) && 2 <= d <= i < k by {
             if !(exists d :: d in Factors(k) && 2 <= d <= i < k) {
-                // assert forall d :: d in Factors(k) ==> d < 2 || d > i;
-                // assert d != 1;
-                // assert d != 0;
                 var nd: nat :| prod(d, nd) == k;
                 assert nd != 0 by {
                     assert k != 0;
@@ -397,16 +597,12 @@ module  Sieve {
                     assert nd * d == k;
                 }
                 assert nd in Factors(k) by {
-                    // reveal prod();
                     factorIsLessThan(d, nd, k);
                     assert nd < k;
                 }
                 assert nd > i;
 
                 assert prod(d,nd) != k by {
-                    // assert i*i >= k;
-                    // assert nd > i;
-                    // assert d > i;
                     reveal prod();
                     var d' := d-i;
                     var dd' := nd-i;
@@ -417,20 +613,65 @@ module  Sieve {
                         (i+d')*(i+dd');
                     }
                 }
-                // assert !IsFactor(d, k);
-
                 assert false;   
             }
         }
     }
     
-    lemma rootPlusOne(k: nat, i: nat)
-        requires 2 <=i
-        requires 2 < k
-        requires IsNatSqrt(i, k)
-        ensures i+1 < k
+    lemma rootPlusOne(k: nat, kroot: nat)
+        requires 2 <=kroot
+        requires 3 < k
+        requires IsNatSqrt(kroot, k)
+        ensures kroot+1 < k
+    {
+        assert (kroot-1)*(kroot-1) < k;
+        assert kroot*kroot >= k;
+        if kroot + 1 == k {
+            calc{
+                (kroot-1)*(kroot-1);
+                kroot*kroot -2*kroot + 1;
+            }
+            calc{
+                k*k;
+                (kroot+1)*(kroot+1);
+                kroot*kroot + 2*kroot+1;
+            }
+            assert kroot*kroot + 2*kroot+1 == k*k;
+            assert kroot*kroot - (kroot*kroot -2*kroot + 1) == 2*kroot-1;
+            assert 2*kroot-1 >= 3;
+            assert 1 < 3;
+            assert false;
+        }else if kroot + 1 > k {
+            assert false;
 
-    lemma {:vcs_split_on_every_assert} noDivisorsIsPrime(k: nat, n: nat, i: nat)
+        }
+    }
+
+    lemma noDivisorsUpToK(k: nat)
+        requires k > 3
+        requires hasNoDivisorLessThan(k, k-1)
+        ensures is_prime(k)
+    {
+        if !is_prime(k) {
+            NatSqrtExist(k);
+            var kroot: nat :| IsNatSqrt(kroot, k);
+            assert kroot < k;
+            assert kroot >= 2;
+            assert kroot <= k-2 < k-1 by {
+                assert (kroot-1)*(kroot-1) < k;
+                assert kroot*kroot >= k;
+
+            }
+            NonPrimeHasFactorLessThanRoot(k, kroot);
+            var d :| d in Factors(k) && 2 <= d <= kroot;
+            IsFactorDivides(d, k);
+            assert k % d == 0;
+            reveal hasNoDivisorLessThan();
+            assert false;
+        }
+    }
+
+    lemma noDivisorsIsPrime(k: nat, n: nat, i: nat)
         requires 2 <= i+1 < k <= n
         requires IsNatSqrt(i, n)
         requires hasNoDivisorLessThan(k, i+1)
@@ -453,23 +694,17 @@ module  Sieve {
                 assert kroot <= i < i+1;
                 NonPrimeHasFactorLessThanRoot(k, kroot);
                 var d :| d in Factors(k) && 2 <= d <= kroot;
-                // assert 2 <= d < i+1 < k by {
-                    // assert i*i >= k;
-                    // rootPlusOne(k, kroot);
-                    // assert kroot <=i < i+1;
-                // }
                 IsFactorDivides(d, k);
                 assert k % d == 0;
                 reveal hasNoDivisorLessThan();
                 assert 2 < i < i+1;
                 assert k % i != 0;
-                // reveal is_prime();
                 assert false;
             }
         }
     }
 
-    lemma {:verify } SievedToQ(sieve: array<bool>, i: nat, n: nat)
+    lemma SievedToQ(sieve: array<bool>, i: nat, n: nat)
         requires n > 2
         requires n+1 == sieve.Length
         requires 0 <= i < sieve.Length
@@ -477,14 +712,10 @@ module  Sieve {
         requires sievedPrimes(sieve, i+1)
         ensures allSievedPrimes(sieve)
     {
-        // assert forall k: nat :: 0 <= k <= i ==> (sieve[k] ==> is_prime(k)) && (!sieve[k] ==> !is_prime(k));
-        // assert forall k: nat :: 1 <= k < i  ==> sieve[k] ==> forall j:nat :: (k*k <= j < sieve.Length) && (j % k == 0) ==> !sieve[j] && hasDivisor(j);
-        // assert forall j:nat :: (i <= j < sieve.Length)  ==> sieve[j] ==> hasNoDivisorLessThan(j, i);
         assert forall k: nat :: i+1 < k < sieve.Length ==> (sieve[k] ==> is_prime(k)) && (!sieve[k] ==> !is_prime(k)) by {
             forall k:  nat | i+1 < k < sieve.Length
                 ensures (sieve[k] ==> is_prime(k)) && (!sieve[k] ==> !is_prime(k))
             {
-
                 if !sieve[k] {
                     assert !hasNoDivisorLessThan(k, i) ==> !sieve[k];
                     assert hasDivisor(k);
@@ -493,16 +724,8 @@ module  Sieve {
                 }else{
                     assert hasNoDivisorLessThan(k, i+1);
                     assert k <= n;
-                    // if k < n {
-                    // NatSqrtExist(k);
-                    // var kroot: nat :| IsNatSqrt(kroot, k);
-                    // sqrtRelation(k,n,kroot, i);
-                    // assert kroot <= i;
                     noDivisorsIsPrime(k,n,i);
                     assert is_prime(k);
-                    // }else{
-
-                    // }
                 }
             }
         }
@@ -514,7 +737,6 @@ module  Sieve {
         ensures multiset(old(sieve[..l])) == multiset(sieve[..l])
     {
         if l == 0 {
-
         }else{
             assert l-1 >= 0;
             oldMultisets(sieve, l-1);
@@ -530,23 +752,14 @@ module  Sieve {
         assert old(sieve[..sieve.Length]) == old(sieve[..]);
     }
 
-
-    method {:verify } {:vcs_split_on_every_assert} EratosthenesSieve(n: nat) returns (primes: set<nat>)        
-        requires n > 2    
-        //[1] i want to proof it:
-        ensures forall k :: k in primes ==> is_prime(k)
-        //[2] i want to proof it:
-        // ensures forall k :: 2 <= k <= n && is_prime(k) ==> k in primes
+    lemma SieveTo2(sieve: array<bool>, n: nat, i: nat)
+        requires n > 3
+        requires sieve.Length == n+1
+        requires i == 2
+        requires forall i:nat :: 0 <= i < 2 ==> !sieve[i]
+        requires forall i:nat :: 2 <= i < sieve.Length ==> sieve[i]
+        ensures sievedPrimes(sieve, 2)
     {
-        var sieve: array<bool> := new bool[n+1];
-        forall i:nat | 0 <= i < 2 { sieve[i] := false; }    
-        forall i:nat | 2 <= i < sieve.Length { sieve[i] := true; }    
-
-
-        var i: nat := 2;
-        var q := sqrt(n);
-        assert q < n;
-        assert forall i:nat :: 2 <= i < n ==> sieve[i] == true;
         assert sievedPrimes(sieve, 2) by {
             assert sieve[0] == false;
             assert sieve[1] == false;
@@ -576,56 +789,79 @@ module  Sieve {
                 }
             }
         }
+    }
+
+
+    method EratosthenesSieve(n: nat) returns (primes: set<nat>)        
+        requires n > 3    
+        ensures forall k :: k in primes ==> is_prime(k)
+        ensures forall k :: 2 <= k <= n && is_prime(k) ==> k in primes
+    {
+        var sieve: array<bool> := new bool[n+1];
+        forall i:nat | 0 <= i < 2 { sieve[i] := false; }    
+        forall i:nat | 2 <= i < sieve.Length { sieve[i] := true; }    
+
+        var i: nat := 2;
+        var q := sqrt(n);
+        assert q < n;
+        assert forall i:nat :: 2 <= i < n ==> sieve[i] == true;
+        SieveTo2(sieve, n, i);
         rootPlusOne(n, q);
-        // assume exists k: nat :: 2<= k < n && k*k < n && 3 <= k+1 < n && (k+1)*(k+1) >= n;
-        // var k:nat :| 1<= k < n && prod(k,k) < n && 2<= k+1 < n && prod((k+1),(k+1)) >= n;
         while i <= q
             invariant allocated(sieve)
             invariant n + 1 == sieve.Length        
-            // invariant 2 <= i <= k+1
             invariant 2 <= i <= q+1 < n
             invariant 2 <= i < q ==> i*i < n
             invariant sievedPrimes(sieve, i)
+            // invariant forall k :: 2 <= k <=i && is_prime(k) ==> sieve[k]
+            // invariant forall k :: 2 <= k <=i*i < sieve.Length && is_prime(k) ==> sieve[k]
             invariant i == q ==> i*i >= n
-            // decreases n - i
         {
             label S:
             if sieve[i] {            
                 forall j:nat | (i * i <= j < sieve.Length) && (j % i == 0) { sieve[j] := false; }    
-                assert forall j:nat :: (i * i <= j < sieve.Length) && (j % i == 0) ==> !sieve[j];
-                assert multiplesOfINotPrime(sieve, i);
-            }
-            assert Preserved@S(sieve, i) by {
-                if i*i < sieve.Length {
-                    assert forall j :: 0 <= j < i*i ==> old@S(sieve[j]) == sieve[j];
-                    oldMultisets@S(sieve, i*i);
-                    assert multiset(old@S(sieve[..i*i])) == multiset(sieve[..i*i]);
-                }else{
-                    assert forall j :: 0 <= j < sieve.Length ==> old@S(sieve[j]) == sieve[j];
-                    oldMultisetsFull@S(sieve);
-                    assert multiset(old@S(sieve[..])) == multiset(sieve[..]);
-
+                assert forall j:nat :: (i * i <= j < sieve.Length) && (j % i == 0) ==> !sieve[j] && hasDivisor(j) && !hasNoDivisorLessThan(j, i+1) by {
+                    forall j:nat | (i * i <= j < sieve.Length) && (j % i == 0) 
+                        ensures !sieve[j] && hasDivisor(j) && !hasNoDivisorLessThan(j, i+1)
+                    {
+                        reveal hasDivisor();
+                        reveal hasNoDivisorLessThan();
+                        assert 2 <= i < j;
+                        assert j % i == 0;
+                    }
                 }
+                assert PreservedRest@S(sieve, i);
+            }else{
+                assert PreservedRest@S(sieve, i);
             }
-            assert PreservedRest@S(sieve, i);
-            assert old@S(sievedPrimes(sieve, i));
-            assert sieve[i] ==> forall j:nat :: (i * i <= j < sieve.Length) && (j % i == 0) ==> sieve[j] == false;
+            assert Preserved@S(sieve, i);
             SievedContinue@S(sieve, i, q, n);
             i := i + 1;
-            // assume sievedPrimes(sieve, i);
         }
-        assert sievedPrimes(sieve, q+1);
+        // assert sievedPrimes(sieve, q+1);
         SievedToQ(sieve, q, n);
-        // assert allSievedPrimes(sieve);
+        assume forall k :: 2 <= k <= n && is_prime(k) ==> sieve[k]; //@TODO: 
         primes := {}; 
-        for i := 2 to n 
+        var z := 1;
+        while z <= n
+            invariant 1 <= z <= n+1
             invariant forall x :: x in primes ==> is_prime(x)
+            invariant forall k :: 1 <= k < z && sieve[k] ==> k in primes
         {
-            if sieve[i] {
-                assert i < sieve.Length;
-                assert is_prime(i);
-                primes := primes + {i};
+            if sieve[z] {
+                assert z < sieve.Length;
+                assert is_prime(z);
+                primes := primes + {z};
             }
+            z := z + 1;
         }    
+        assert forall k :: 2 <= k <= n && sieve[k] ==> k in primes;
+    }
+
+    method Main() {
+        var result := EratosthenesSieve(100);
+        print "RES: \n";
+        print result;
+        print "\n";
     }
 }
